Mathlib style

AutomataInLean/DFA.lean
@@ -15,38 +15,38 @@ theorem invert_accepts_iff (x : List α) : x ∈ (invert M).accepts ↔ x ∉ M.
   apply invert_accept_iff
 
 -- Cartesian product of two DFAs with an arbitrary acceptance condition
-def cartesian_product (p : Prop -> Prop -> Prop) (M1 : DFA α σ) (M2 : DFA α σ') : DFA α (σ × σ') := {
-  step := fun ⟨s1, s2⟩ a => (M1.step s1 a, M2.step s2 a),
-  start := (M1.start, M2.start),
-  accept := {s | p (s.fst ∈ M1.accept) (s.snd ∈ M2.accept)}
+def cartesian_product (p : Prop → Prop → Prop) (M₁ : DFA α σ) (M₂ : DFA α σ') : DFA α (σ × σ') := {
+  step := fun ⟨s₁, s₂⟩ a => (M₁.step s₁ a, M₂.step s₂ a),
+  start := (M₁.start, M₂.start),
+  accept := {s | p (s.fst ∈ M₁.accept) (s.snd ∈ M₂.accept)}
 }
 
-theorem cartesian_product_accept_iff (p : Prop -> Prop -> Prop) (M1 : DFA α σ) (M2 : DFA α σ') (s : σ × σ') :
-  s ∈ (cartesian_product p M1 M2).accept ↔ p (s.fst ∈ M1.accept) (s.snd ∈ M2.accept) := by
+theorem cartesian_product_accept_iff (p : Prop → Prop → Prop) (M₁ : DFA α σ) (M₂ : DFA α σ') (s : σ × σ') :
+    s ∈ (cartesian_product p M₁ M₂).accept ↔ p (s.fst ∈ M₁.accept) (s.snd ∈ M₂.accept) := by
   simp [cartesian_product]
 
-theorem cartesian_product_eval_from (p : Prop -> Prop -> Prop) (M1 : DFA α σ) (M2 : DFA α σ') (x : List α) :
-  ∀ s : σ × σ',
-  (cartesian_product p M1 M2).evalFrom s x = ⟨M1.evalFrom s.1 x, M2.evalFrom s.2 x⟩ := by
+theorem cartesian_product_eval_from (p : Prop → Prop → Prop) (M₁ : DFA α σ) (M₂ : DFA α σ') (x : List α) :
+    ∀ s : σ × σ',
+    (cartesian_product p M₁ M₂).evalFrom s x = ⟨M₁.evalFrom s.1 x, M₂.evalFrom s.2 x⟩ := by
   dsimp [DFA.evalFrom, cartesian_product]
   induction' x with a x' ih
   · simp
   · intro s
     simp [List.foldl, ih, DFA.step]
 
-theorem cartesian_product_accepts_iff (p : Prop -> Prop -> Prop) (M1 : DFA α σ) (M2 : DFA α σ') (x : List α) :
-  x ∈ (cartesian_product p M1 M2).accepts ↔ p (x ∈ M1.accepts) (x ∈ M2.accepts) := by
+theorem cartesian_product_accepts_iff (p : Prop → Prop → Prop) (M₁ : DFA α σ) (M₂ : DFA α σ') (x : List α) :
+    x ∈ (cartesian_product p M₁ M₂).accepts ↔ p (x ∈ M₁.accepts) (x ∈ M₂.accepts) := by
   simp [DFA.accepts]
   simp [DFA.acceptsFrom, cartesian_product_eval_from]
   simp [cartesian_product]
   repeat rw [Set.mem_setOf_eq]
 
-def intersect (M1 : DFA α σ) (M2 : DFA α σ') : DFA α (σ × σ') := cartesian_product And M1 M2
+def intersect (M₁ : DFA α σ) (M₂ : DFA α σ') : DFA α (σ × σ') := cartesian_product And M₁ M₂
 
-theorem intersect_accept_iff (M1 : DFA α σ) (M2 : DFA α σ') (s : σ × σ') :
-  s ∈ (intersect M1 M2).accept ↔ s.fst ∈ M1.accept ∧ s.snd ∈ M2.accept := by
+theorem intersect_accept_iff (M₁ : DFA α σ) (M₂ : DFA α σ') (s : σ × σ') :
+    s ∈ (intersect M₁ M₂).accept ↔ s.fst ∈ M₁.accept ∧ s.snd ∈ M₂.accept := by
   simp [intersect, cartesian_product_accept_iff]
 
-theorem intersect_accepts_iff (M1 : DFA α σ) (M2 : DFA α σ') (x : List α) :
-  x ∈ (intersect M1 M2).accepts ↔ x ∈ M1.accepts ∧ x ∈ M2.accepts := by
+theorem intersect_accepts_iff (M₁ : DFA α σ) (M₂ : DFA α σ') (x : List α) :
+    x ∈ (intersect M₁ M₂).accepts ↔ x ∈ M₁.accepts ∧ x ∈ M₂.accepts := by
   simp [intersect, cartesian_product_accepts_iff]
